- **substitution** - $\frac{E}{E[v \coloneqq  F]}$
- **reflexivity** - $x \equiv x$
- **symmetry** - $(x \equiv y) \equiv (y \equiv x)$
- **transitivity** - $\frac{X \equiv Y, Y \equiv Z}{X \equiv Z}$
- **Leibnitz rule of interference** - $\frac{X \equiv Y}{E[z \coloneqq X] \equiv E[z \coloneqq Y]} \forall E$

Equivalence \equiv and true
= is conjunctional: b = c = d is b = c \land c = d
\equiv is associative: b \equiv c \equiv d is (b \equiv c) \equiv d
(3.1) Ax. Associativity of \equiv ((p \equiv q) \equiv r) \equiv (p \equiv (q \equiv r))
(3.2) Ax. Symmetry of \equiv p \equiv q \equiv q \equiv p (p \equiv q) \equiv (q \equiv p)
p \equiv (q \equiv q \equiv p) (p \equiv q \equiv q) \equiv p
(3.3) Ax. Identity of \equiv true \equiv q \equiv q (true \equiv q) \equiv q
true \equiv (q \equiv q)
(3.4) Th. true
(3.5) Th. Reflexivity of \equiv p \equiv p

Negation \lnot , Inequivalence 6\equiv , and false
(3.8) Ax. Definiton of false false \equiv \lnot true
(3.9) Ax. Dist. of \lnot  over \equiv \lnot (p \equiv q) \equiv \lnot p \equiv q
(3.10) Ax. Def. of 6\equiv (p 6\equiv q) \equiv \lnot (p \equiv q)
(3.11) Th. \lnot p \equiv q \equiv p \equiv \lnot q
(3.12) Th. Double Negation \lnot \lnot p \equiv p
(3.13) Th. Negation of false \lnot false \equiv true
(3.14) Th. (p 6\equiv q) \equiv \lnot p \equiv q
(3.15) Th. \lnot p \equiv p \equiv false
(3.16) Th. Symmetry of 6\equiv (p 6\equiv q) \equiv (q 6\equiv p)
(3.17) Th. Associativity of 6\equiv ((p 6\equiv q) 6\equiv r) \equiv (p 6\equiv (q 6\equiv r))
(3.18) Th. Mutual Associativity ((p 6\equiv q) \equiv r) \equiv (p 6\equiv (q \equiv r))
(3.19) Th. Mutual Interchangability p 6\equiv q \equiv r \equiv p \equiv q 6\equiv r
(3.20) Fact About Sequences P0 \equiv P1 \equiv \dots \equiv Pn is true
exactly when an even number of Pi are false

Disjunction \lor 
(3.24) Ax. Symmetry of \lor p \lor q \equiv q \lor p
(3.25) Ax. Associativity of \lor (p \lor q) \lor r \equiv p \lor (q \lor r)
(3.26) Ax. Idempotency of lor p \lor p \equiv p
(3.27) Ax. Dist. of \lor over \equiv p \lor (q \equiv r) \equiv p \lor q \equiv p \lor r
(3.28) Ax. Excluded Middle p \lor \lnot p a value must always be
true or not true, it cannot be both!
(3.29) Th. Zero of \lor p \lor true \equiv true
(3.30) Th. Identity of \lor p \lor false \equiv p
(3.31) Th. Dist. of \lor over \lor p \lor (q \lor r) \equiv (p \lor q) \lor (p \lor r)
(3.32) Th. p \lor q \equiv p \lor \lnot q \equiv p
(9.9) (\forall x|R : P \equiv Q) \implies  ((\forall x|R : P) \equiv (\forall x|R : Q))
(9.10) Range Weak./Strength. (\forall x|Q \lor R : P) \implies  (\forall x|Q : P)
(9.11) Body Weak./Strength. (\forall x|R : P \land Q) \implies  (\forall x|R : P)
(9.12) Monocity of \forall 
(\forall x|R : Q \implies  P) \implies  ((\forall x|R : Q) \implies  (\forall x|R : P))
(9.13) Instantiation (\forall x| : P) \implies  P[x := E]


Conjunction \land 
(3.35) Ax. Golden Rule p \land q \equiv p \equiv q \equiv p \lor q
(p \equiv q) \equiv (p \land q \equiv p \lor q)
(3.36) Ax. Symmetry of \land p \land q \equiv q \land p
(3.37) Ax. Associativity of \land (p \land q) \land r \equiv p \land (q \land r)
(3.38) Ax. Idempotency of \land p \land p \equiv p
(3.39) Ax. Identity of \land p \land true \equiv p
(3.40) Ax. Zero of \land p \land false \equiv false
(3.41) Ax. Dist. of \land over \lor p \land (q \land r) \equiv (p \land q) \land (p \land r)
(3.42) Ax. Contradiction p \land \lnot p \equiv false
(3.43) Th. Absorption a) p \land (p \lor q) \equiv p b) p \lor (p \land q) \equiv p
(3.44) Th. Absorption a) p \land (\lnot p \lor q) \equiv p \land q b)
p \lor (\lnot p \land q) \equiv p \lor q
(3.45) Th. Dist. of \land over \lor p \lor (q \land r) \equiv (p \lor q) \land (p \lor r)
(3.46) Th. Dist. of \land over \lor p \land (q \lor r) \equiv (p \land q) \lor (p \land r)
(3.47) Th. De Morgan a) \lnot (p \land q) \equiv \lnot p \lor \lnot q b)
\lnot (p \lor q) \equiv \lnot p \land \lnot q
(3.48) Th. p \land q \equiv p \land \lnot q \equiv \lnot p
(3.49) Th. p \land (q \equiv r) \equiv p \land q \equiv p \land r \equiv p
(3.50) Th. p \land (q \equiv p) \equiv p \land q
(3.51) Th. Replacement (p \equiv q) \land (r \equiv p) \equiv (p \equiv q) \land (r \equiv q)
(3.52) Ax. Def. of \equiv p \equiv q \equiv (p \land q) \lor (\lnot p \land \lnot q)
(3.53) Ax. Def. of Exclusive or p 6\equiv q \equiv (\lnot p \land q) \lor (p \land \lnot q)
(3.55) Th.
(p \lor q) \lor r \equiv p \equiv q \equiv r \equiv p \lor q \equiv q \lor r \equiv r \lor p \equiv p \lor q \lor r

Implication
Note: for p \implies  q, q \implies  p is the converse, \lnot q \implies  \lnot p is the
contrapositive and \lnot p \implies  \lnot q is the inverse.
(3.57) Ax. Def. of Implication p \implies  q \equiv p \lor q \equiv q
(3.58) Ax. Def. of Consequence p \Leftarrow q \equiv q \implies  p
(3.59) Th.Alternative Def. of Implication p \implies  q \equiv \lnot p \lor q
(3.60) Th. Alternative Def. of Implication p \implies  q \equiv p \land q \equiv p
(3.61) Th. Contrapositive p \implies  q \equiv \lnot q \implies  \lnot p
(3.62) Th. p \implies  (q \equiv r) \equiv p \land q \equiv p \land r
(3.63) Th. Dist. of \implies  over \equiv p \implies  (q \equiv r) \equiv p \implies  q \equiv p \implies  r
(3.64) Th. p \implies  (q \implies  r) \equiv (p \implies  q) \implies  (p \implies  r)
(3.65) Th. Shunting p \land q \implies  r \equiv p \implies  (q \implies  r)
(3.66) Th. p \land (p \implies  q) \equiv p \land q
(3.67) Th. p \land (q \implies  p) \equiv p
(3.68) Th. p \lor (p \implies  q) \equiv true
(3.69) Th. p \lor (q \implies  p) \equiv q \implies  p
(3.70) Th. p \lor q \implies  p \land q \equiv p \equiv q
(3.71) Th. Reflexivity of \implies  p \implies  p \equiv true
(3.72) Th. Right zero of \implies  p \implies  true \equiv true
(3.73) Th. Left identity of \implies  true \implies  p \equiv p
(3.74) Th. p \implies  false \equiv \lnot p
(3.75) Th. false \implies  p \equiv true
(3.76) Th. Weak./Strength. 
a) p \implies  p \lor q 
b) p \land q \implies  p 
c) p \land q \implies  p \lor q 
d) p \lor (q \land r) \implies  p \lor q 
e) p \land q \implies  p \land (q \lor r)
(3.77) Th. Modus ponens p \land (p \implies  q) \implies  q
(3.78) Th. Case Analysis (p \implies  r) \land (q \implies  r) \equiv (p \lor q \implies  r)
(3.79) Th. Case Analysis (p \implies  r) \land (\lnot p \implies  r) \equiv r
(3.80) Th. Mutual Implication (p \implies  q) \land (q \implies  p) \equiv p \equiv q
(3.81) Th. Antisymmetry (p \implies  q) \land (q \implies  p) \implies  (p \equiv q)
(3.82) Th. Transitivity 
a) (p \implies  q) \land (q \implies  r) \implies  (p \implies  r)
b) (p \equiv q) \land (q \implies  r) \implies  (p \implies  r)
c) (p \implies  q) \land (q \equiv r) \implies  (p \implies  r)

Leibniz as an Axiom
(3.83) Ax. Leibniz (e = f) \implies  (E_e^z = E_f^z
) where E is any exp.
(3.84) Th. Sub. a) (e = f) \land E_e^z \equiv (e = f) \land E_f^z
b)
(e = f) \implies  E_e^z \equiv (e = f) \implies  E_f^z
c)
q \land (e = f) \implies  E_e^z \equiv q \land (e = f) \implies  E_f^z
(3.85) Th. Replace by true 
a) p \implies  E_p^z \equiv p \implies  E_{true}^z 
b) q \land p \implies  E_p^z \equiv q \land p \implies  E_{true}^z
(3.86) Th. Replace by false 
a) E_p^z \implies  p \equiv E_{false}^x \implies  p 
b) E_p^z \implies  p \lor q \equiv E_{false}^x \implies  p \lor q
(3.87) Th. Replace by true p \land E_p^z \equiv p \land E_{true}^z
(3.88) Th. Replace by false p \lor E_p^z \equiv p \lor E_{false}^z
(3.89) Th. Shannon E_p^z \equiv (p \land E_{true}^z) \lor (\lnot p \land E_{false}^z)
(4.1) p \implies  (q \implies  p)
(4.2) Monotonicity of \lor (p \implies  q) \implies  (q \lor r \implies  q \land r)
(4.3) Monotonicity of \land (p \land q) \implies  (p \land r \implies  q \land r)
. For the following rules, assume ∗ operator is symmetric,
associative and has identity u
(8.13) Ax., Empty range (*x|false : P) = u (u is the identity
of * )
(8.14) Ax., One-point rule Provided \lnot occurs('x','E'),
(*x|x = E : P) = P[x := E]
(8.15) Ax., Dist. Provided each Quant. is defined,
(*x|R : P) * (*x|R : Q) = (*x|R : P * Q)
(8.16) Ax., Range split Provided R \land S \equiv false and each
Quant. is defined, (*x|R \lor S : P) = (*x|R : P) * (*x|S : P)
(8.17) Ax., Range split Provided each Quant. is defined,
(*x|R \lor S : P) * (*x|R \land S : P) = (*x|R : P) * (*x|S : P) (8.18)
Ax., Range split for idempotent * Provided each Quant. is
defined, (*x|R \lor S : P) = (*x|R : P) * (*x|S : P)
(8.19) Ax., Interchange of dummies Provided each Quant. is
defined, \lnot occurs('y','R')and \lnot occurs('x','Q'), (*x|R : (*y|Q : P)) = (*y|Q : (*x|R : P))
(8.20) Ax., Nesting Provided \lnot occurs(
'y
'
,
' R'
),
(*x, y|R \land Q : P) = (*x|R : (*y|Q : P))
(8.21) Ax., Dummy renaming Provided \lnot occurs(
'y
'
,
' R, P'
),
(*x|R : P) = (*y|R[x := y] : P[x := y])
(8.22) Change of dummy Provided \lnot occurs(
'y
'
,
' R, P'
) and f
has an inverse, (*x|R : P) = (*y|R[x := f.y] : P[x := f.y])
(8.23) Th. Split off term For n : N and dummies i : N,
(*i|0 ≤ i ≤ n + 1 : P) = (*i|0 ≤ i < n : P) * P[i := n]
(*i|0 ≤ i ≤ n + 1 : P) = P[i := 0] * (*i|0 < i < n + 1 : P)
 
Predicate Calculus
Universal Quantification
(9.2) Ax., Trading (\forall x|R : P) \equiv (\forall x| : R \implies  P)
(9.3) Trading (a) (\forall x|R : P) \equiv (\forall x| : \lnot R \lor P) (b)
(\forall |R : P) \equiv (\forall | : R \land P \equiv R) (c)
(\forall x|R : P) \equiv (\forall x| : R \lor P \equiv P)
(9.4) Trading (a) (\forall x|Q \land R : P) \equiv (\forall x|Q : R \implies  P) (b)
(\forall x|Q \land R : P) \equiv (\forall x|Q : \lnot R \lor P) (c)
(\forall x|Q \land R : P) \equiv (\forall x|Q : R \land P \equiv R) (d)
(\forall x|Q \land R : P) \equiv (\forall x|Q : R \lor P \equiv P)
(9.5) Ax., Dist. of \lor over \forall  Provided \lnot occurs(
'x
'
,
' P
'
),
P \lor (\forall x|R : Q) \equiv (\forall x|R : P \lor Q)
(9.6) Provided \lnot occurs(
'x
'
,
' P
'
), (\forall x|R : P) \equiv P \lor (\forall x| : \lnot R)
(9.7) Dist. of \land over \forall 
\lnot (\forall x| : \lnot R) \implies  ((\forall x|R : P \land Q) \equiv P \land (\forall x|R : Q))
(9.8) (\forall x|R : true) \equiv true

Existential Quantification
(9.17) Ax., Generalized De Morgan (∃x|R : P) \equiv \lnot (\forall x|R : \lnot P)
(9.18) Generalized De Morgan (a) \lnot (∃x|R : \lnot P) \equiv (\forall x|R : P)
(b)\lnot (∃x|R : P) \equiv (\forall x|R : \lnot P) (c)(∃x|R : \lnot P) \equiv \lnot (\forall x|R : P)
(9.19) Trading (∃x|R : P) \equiv (∃x| : R \land P)
(9.2') Trading (∃x|Q \land R : P) \equiv (∃x|Q : R \land P)
(9.21) Dist. of \land over ∃ Provided \lnot occurs(
'x
'
,
' P
'
),
P \land (∃x|R : Q) \equiv (∃x|R : P \land Q)
(9.22) Provided \lnot occurs(
'x
'
,
' P
'
), (∃x|R : P) \equiv P \land (∃x| : R)
(9.23) Dist. of \lor over ∃ Provided \lnot occurs(
'x
'
,
' P
'
),
(∃x| : R) \implies  ((∃x|R : P \lor Q) \equiv P \lor (∃x|R : Q))
(9.24) (∃x|R : false) \equiv false
(9.25) Range Weak./Strength. (∃x|R : P) \implies  (∃x|Q \lor R : P)
(9.26) Body Weak./Strength. (∃x|R : P) \implies  (∃x|R : P \lor Q)
(9.27) Monocity of ∃
(\forall x|R : Q \implies  P) \implies  ((∃x|R : Q) \implies  (∃x|R : P))
(9.28) ∃-Introduction P[x := E] \implies  (∃x| : P)
(9.29) Interchange of Quant. Provided \lnot occurs(
0y
0
,
0 R0
) and
\lnot occurs ∗
0 x
0
,
0 Q0
), (∃x|R : (\forall y : Q : P)) \implies  (\forall y|Q : (∃x|R : P))
