# Propositional Logic

order of precedence

symbol  |  order
:---: | :---:
$$()$$ | 0
$$\forall, \exists$$ | 1
$$\lnot$$ | 2
$$\land$$ | 3
$$\lor$$ | 4
$$\implies$$ | 5
$$\leftrightarrow$$ | 6

## definitions

- **proposition** - a declarative sentence that is either true or false
- **consistent** - a list of propositions is consistent if it is possible to assign truth values to the proposition variables so that each proposition is true
- **tautology** - a proposition which is always true ex. $$ a \lor \lnot b $$
- **contradiction** - a proposition which is always false ex. $$ a \land \lnot b $$
- **contingency** - a proposition which is neither a tautology nor a contradiction, such as $$ a $$
- **logical equivalence** - two compound propositions a and b are logically equivalent if $$ a \leftrightarrow b $$ is a tautology. write as $$ a \iff b $$ or $$ a \equiv b $$, their truth tables have to have the same value

### negation / $$\lnot$$

<details>
<summary>truth table</summary>

$$a$$ | $$\neg a$$ |
:-: | :-: |
T | F |
F | T |
</details>


### conjunction / and / $$\land$$
<details>
<summary>truth table</summary>

$$a$$ | $$b$$ | $$a \land b$$ |
:-: | :-: | :-: |
T | T | T |
T | F | F |
F | T | F |
F | F | F |
</details>

### disjunction / or / $$\lor$$
<details>
<summary>truth table</summary>

$$a$$ | $$b$$ | $$a \lor b$$ |
:-: | :-: | :-: |
T | T | T |
T | F | T |
F | T | T |
F | F | F |
</details>

### exclusive disjunction / xor / $$\oplus$$
<details>
<summary>truth table</summary>

$$a$$ | $$b$$ | $$a \oplus b$$ |
:-: | :-: | :-: |
T | T | F |
T | F | T |
F | T | T |
F | F | F |
</details>

### implication / $$\rightarrow$$

can be written as 
- if A then B
- if A, B
- B unless Â¬A
- B if A
- B whenever A
- B follows from A
- A implies B
- A only if B
- B when A
- A is sufficient for B 
- B is necessary for A 
- a necessary condition for A is B
- B is a necessary condition for A 
- a sufficient condition for B is A
- A is a sufficient condition for B 

<details>
<summary>truth table</summary>

$$a$$ | $$b$$ | $$a \rightarrow b$$ |
:-: | :-: | :-: |
T | T | T |
T | F | F |
F | T | T |
F | F | T |
</details>

### biconditional / $$\leftrightarrow$$ / $$\equiv$$

- if and only if
- a is necessary and sufficient for b
- if a then b, and conversely
- a iff b

<details>
<summary>truth table</summary>

$$a$$ | $$b$$ | $$a \leftrightarrow b$$ |
:-: | :-: | :-: |
T | T | T |
T | F | F |
F | T | F |
F | F | T |
</details>

## De Morgan's Laws

$$ \lnot (p \land q) \equiv \lnot p \lor \lnot q $$, and $$ \lnot (p \lor q) \equiv \lnot p \land \lnot q $$

$$\lnot \forall x P(x) \equiv \exist x \lnot P(x)$$

$$\lnot \exist x P(x) \equiv \forall x \lnot P(x)$$ 

# Key Logical Equivalences
- **Identity Laws** - $$p\land T\equiv p$$, and $$p\lor F\equiv p$$
- **Domination Laws** - $$p\lor T\equiv T$$, and $$p\land F\equiv F$$
- **Idempotent Laws** - $$p\lor p\equiv p$$, and $$p\land p\equiv p$$
- **Double Negation Law** - $$\neg (\neg p)\equiv p$$
- **Negation Laws** - $$p\lor \neg p\equiv T$$, and $$p\land \neg p\equiv F$$
- **Commutative Laws** - $$p\lor q\equiv q\lor p$$, and $$p\land q\equiv q\land p$$
- **Associative Laws** - $$(p\land q)\land r\equiv p\land (q\land r)$$, and $$(p\lor q)\lor r\equiv p\lor (q\lor r)$$
- **Distributive Laws** - $$(p\lor(q\land r))\equiv(p\lor q)\land (p\lor r)$$, and $$(p\land(q\lor r))\equiv(p\land q)\lor (p\land r)$$
- **Absorption Laws** - $$p\lor(p\land q)\equiv p$$, and $$p\land(p\lor q)\equiv p$$

# equivalence proofs

![proof](./media/1_propositional_logic_1.png)

## converse, contrapositive, and inverse

from $$ a \rightarrow b $$ we can form new conditional statements
- $$ b \rightarrow a $$ is the converse
- $$ \lnot b \rightarrow \lnot a $$  is the contrapositive
- $$ \lnot a \rightarrow \lnot b $$  is the inverse

# Predicate Logic

- **variables** - x,y,z
- **Predicates** - P(x), M(x)
- **Quantifiers** - symbols to express meaning of english words/statements
    - **universal quantifier** $$\forall$$ (\forall) - for all / for every ex. $$\forall x P(x)$$ asserts P(x) is true for *every* x in the domain
    - **existential quantifier** $$\exists$$ (\exists) - there exists ex. $$\exists x P(x)$$ asserts P(x) is true for *some* x in the domain
- **propositional functions** - generalizations of propositions. contain variables and a predicate. variables can be replaced by elements from their domain
    - example: let "x + y = z" be donated by R(x,y,z). R(2,-1,5) is false, R(3,4,7) is true
- **compound expressions** - $$P(x) \land P(y)$$


## Nested quantifiers

every real number has an inverse:
$$\forall x \exists y (x + y = 0)$$

### nested loops
to see if $$\forall x \forall y P (x,y)$$ is true, loop through all values of y, in inner loop go through all values of x

if the domain of the variables are infinite, this process can not be carried out

## order of quantifiers
example
 let $$ P(x,y)$$ be the statement $$x + y = y + x$$. Assume that U is the real numbers. Then  $$\forall x \forall y P (x,y)$$ and  $$\forall y \forall x P (x,y)$$ have the same truth value

`TODO: fix`
let $$ Q(x,y)$$ be the statement $x + y = o$$. Then $$\forall x \exists y Q (x,y)$$ is true, $$\exists y \forall x Q (x,y)$$ is true

let U be the real numbers
Define $$P(x,y): x \cdot y = 0$$
- $$\forall x \forall y P (x,y)$$ = False
- $$\forall x \exists y P (x,y)$$ = True
- $$\exists x \forall y P (x,y)$$ = True
- $$\exists x \exists y P (x,y)$$ = True

Define $$P(x,y): \frac{x}{y} = 1$$
- $$\forall x \forall y P (x,y)$$ = False
- $$\forall x \exists y P (x,y)$$ = False x = 0
- $$\exists x \forall y P (x,y)$$ = False y != 0
- $$\exists x \exists y P (x,y)$$ = True

english
- $$\forall x \forall y P (x,y)$$ 
- $$\forall x \forall y P (x,y)$$ P(x,y) is true for every pair x,y

- $$\exists x \forall y P (x,y)$$ For every x there is a y for which P(x,y) is true
- $$\forall x \exists y P (x,y)$$ There is an x for which P(x,y) is true for every y

- $$\exists x \exists y P (x,y)$$ 
- $$\exists y \exists x P (x,y)$$ There is a pair x,y for which P(x,y) is true
